Reap/Test.lean
@@ -2,4 +2,5 @@ import Reap.Test.PremiseSelection
 import Reap.Test.Tactic.MCTS
 import Reap.Test.Tactic.State
 import Reap.Test.Tactic.Step
+import Reap.Test.Tactic.TreeSearch
 import Reap.Test.TreeSearch.BestFirst
